some work on bv library

tools/Vale/testBV/Larith.fst
@@ -20,46 +20,46 @@ let logxor_uint  (#n:pos) (x:int) (y:int)
            [SMTPat (logxor #n x y)]
   = ()          
 
-// abstract
-// let logand (#n:pos) (x:int) (y:int) : nat64 =
-//   if FStar.UInt.fits x n
-//   && FStar.UInt.fits y n
-//   then FStar.UInt.logand #n x y
-//   else 0
+abstract
+let logand (#n:pos) (x:int) (y:int) : res:nat{res < pow2 n} =
+  if FStar.UInt.fits x n
+  && FStar.UInt.fits y n
+  then FStar.UInt.logand #n x y
+  else 0
 
-// let logand_uint64 (x:int) (y:int)
-//   : Lemma (ensures (FStar.UInt.fits x 64 /\
-//                     FStar.UInt.fits y 64) ==>
-//                     logand x y = FStar.UInt.logand #64 x y)
-//           [SMTPat (logand x y)]
-//   = ()          
+let logand_uint (#n:pos) (x:int) (y:int)
+  : Lemma (ensures (FStar.UInt.fits x n /\
+                    FStar.UInt.fits y n) ==>
+                    logand #n x y = FStar.UInt.logand #n x y)
+          [SMTPat (logand #n x y)]
+  = ()          
 
-// abstract
-// let shift_right (x:int) (y:int) : nat64 =
-//   if FStar.UInt.fits x 64
-//   && y >= 0
-//   then FStar.UInt.shift_right #64 x y
-//   else 0
+abstract
+let shift_right (#n:pos) (x:int) (y:int) : res:nat{res < pow2 n} =
+  if FStar.UInt.fits x n
+  && y >= 0
+  then FStar.UInt.shift_right #n x y
+  else 0
 
-// let shift_right_uint64 (x:int) (y:int)
-//   : Lemma (ensures (FStar.UInt.fits x 64 /\
-//                     0 <= y /\
-//                     y < 64 ==>
-//                     shift_right x y = FStar.UInt.shift_right #64 x y))
-//           [SMTPat (shift_right x y)]
-//   = ()          
+let shift_right_uint (#n:pos) (x:int) (y:int)
+  : Lemma (ensures (FStar.UInt.fits x n /\
+                    0 <= y /\
+                    y < n ==>
+                    shift_right #n x y = FStar.UInt.shift_right #n x y))
+          [SMTPat (shift_right #n x y)]
+  = ()          
 
-// abstract
-// let shift_left (x:int) (y:int) : nat64 =
-//   if FStar.UInt.fits x 64
-//   && y >= 0
-//   then FStar.UInt.shift_left #64 x y
-//   else 0
+abstract
+let shift_left (#n:pos) (x:int) (y:int) : res:nat{res < pow2 n} =
+  if FStar.UInt.fits x n
+  && y >= 0
+  then FStar.UInt.shift_left #n x y
+  else 0
 
-// let shift_left_uint64 (x:int) (y:int)
-//   : Lemma (ensures (FStar.UInt.fits x 64 /\
-//                     0 <= y /\
-//                     y < 64 ==>
-//                     shift_left x y = FStar.UInt.shift_left #64 x y))
-//           [SMTPat (shift_left x y)]
-//   = (
+let shift_left_uint (#n:pos) (x:int) (y:int)
+  : Lemma (ensures (FStar.UInt.fits x n /\
+                    0 <= y /\
+                    y < n ==>
+                    shift_left #n x y = FStar.UInt.shift_left #n x y))
+          [SMTPat (shift_left #n x y)]
+  = ()
